$\Delta = \set{\text{0, roots of $g$}}$


$2s^{-1/2}\arctan\left(\frac{x-s}{s}\right)^{1/2}$


$x^{1/2}(x-1)^{1/2}(x-s)^{3/2}$


$f'(x) = s(s-1) O$+


\begin{equation*}
a_g(s) \frac{ d^g  }{ds^g}[\omega(s)] + \cdots +
ba_1(s) \frac{ d  }{ds}[\omega(s)] +
a_0(s) [\omega(s)]  = 0
\end{equation*}

\begin{equation*}
\begin{split}
\omega(s) = x^{-1/2}(x-1)^{-1/2}(x-s)^{-1/2} dx \\
\omega'(s) = \frac{1}{2} x^{-1/2}(x-1)^{-1/2}(x-s)^{-3/2} dx \\
\omega'(s) = \frac{3}{4} x^{-1/2}(x-1)^{-1/2}(x-s)^{-5/2} dx
\end{split}
\end{equation*}

